Logic/Predicate/FirstOrder/Ultraproduct.lean
@@ -4,25 +4,26 @@ universe u v
 
 section
 
-variable {L : Language.{u}} {μ : Type v} {n : ℕ} {I : Type u}
-  (A : I → Type u) [(ι : I) → Inhabited (A ι)] (s : (ι : I) → Structure₁ L (A ι)) (𝓤 : Ultrafilter I)
+variable {L : Language.{u}} {μ : Type v}
+ {I : Type u} (A : I → Type u) [(ι : I) → Inhabited (A ι)] [s : (ι : I) → Structure₁ L (A ι)] (𝓤 : Ultrafilter I)
 
 namespace Structure₁
 
 structure Uprod (𝓤 : Ultrafilter I) where
   val : (i : I) → A i
 
-def UprodStruc : Structure₁ L (Uprod A 𝓤) where
+instance UprodStruc : Structure₁.{u,u} L (Uprod A 𝓤) where
   func := fun f v => ⟨fun ι => (s ι).func f (fun i => (v i).val ι)⟩
   rel  := fun r v => {ι | (s ι).rel r (fun i => (v i).val ι)} ∈ 𝓤
+
 
 instance [Inhabited I] [(ι : I) → Inhabited (A ι)] : Inhabited (Uprod A 𝓤) := ⟨⟨default⟩⟩
 
 @[simp] lemma func_Uprod {k} (f : L.func k) (v : Fin k → Uprod A 𝓤) :
-    (UprodStruc A s 𝓤).func f v = ⟨fun ι => (s ι).func f (fun i => (v i).val ι)⟩ := rfl
+    func f v = ⟨fun ι => (s ι).func f (fun i => (v i).val ι)⟩ := rfl
 
 @[simp] lemma rel_Uprod {k} (r : L.rel k) (v : Fin k → Uprod A 𝓤) :
-    (UprodStruc A s 𝓤).rel r v ↔ {ι | (s ι).rel r (fun i => (v i).val ι)} ∈ 𝓤 := of_eq rfl
+    rel r v ↔ {ι | (s ι).rel r (fun i => (v i).val ι)} ∈ 𝓤 := of_eq rfl
 
 end Structure₁
 
@@ -31,7 +32,7 @@ open Structure₁
 variable (e : Fin n → Uprod A 𝓤) (ε : μ → Uprod A 𝓤)
 
 lemma val_Uprod (t : SubTerm L μ n) :
-    t.val (UprodStruc A s 𝓤) e ε = ⟨fun ι => t.val (s ι) (fun i => (e i).val ι) (fun i => (ε i).val ι)⟩ :=
+    t.val! (Uprod A 𝓤) e ε = ⟨fun ι => t.val (s ι) (fun i => (e i).val ι) (fun i => (ε i).val ι)⟩ :=
   by induction t <;> simp[*, val_func]
 
 end SubTerm
@@ -48,7 +49,7 @@ lemma val_vecCons_val_eq {z : Uprod A 𝓤} {ι : I} :
   by simp[Matrix.comp_vecCons (Uprod.val · ι), Function.comp]
 
 lemma eval_Uprod {p : SubFormula L μ n} :
-    Eval (UprodStruc A s 𝓤) e ε p ↔ {ι | Eval (s ι) (fun i => (e i).val ι) (fun i => (ε i).val ι) p} ∈ 𝓤 := by
+    Eval! (Uprod A 𝓤) e ε p ↔ {ι | Eval (s ι) (fun i => (e i).val ι) (fun i => (ε i).val ι) p} ∈ 𝓤 := by
   induction p using rec' <;>
   simp[*, Prop.top_eq_true, Prop.bot_eq_false, eval_rel, eval_nrel, SubTerm.val_Uprod]
   case hverum => exact Filter.univ_mem
@@ -68,7 +69,7 @@ lemma eval_Uprod {p : SubFormula L μ n} :
         have : Eval (s ι) (z.val ι :> fun i => (e i).val ι) (fun i => (ε i).val ι) p :=
           by rw [val_vecCons_val_eq]; exact hι
         by_contra hc
-        have : ¬Eval (s ι) (z.val ι :> fun i => (e i).val ι) (fun i => (ε i).val ι) p :=
+        have : ¬Eval! (A ι) (z.val ι :> fun i => (e i).val ι) (fun i => (ε i).val ι) p :=
           Classical.epsilon_spec (p := fun z => ¬(Eval (s ι) (z :> fun i => (e i).val ι) _ p)) ⟨a, hc⟩
         contradiction)
     · intro h x
@@ -88,23 +89,18 @@ lemma eval_Uprod {p : SubFormula L μ n} :
         rw[val_vecCons_val_eq] at this; exact this)
 
 lemma val_Uprod {p : Formula L μ} :
-    Val (UprodStruc A s 𝓤) ε p ↔ {ι | Val (s ι) (fun i => (ε i).val ι) p} ∈ 𝓤 :=
+    Val! (Uprod A 𝓤) ε p ↔ {ι | Val (s ι) (fun i => (ε i).val ι) p} ∈ 𝓤 :=
   by simp[Val, eval_Uprod, Matrix.empty_eq]
 
 end SubFormula
 
-instance zzz [(ι : I) → CStruc L (A ι)] : CStruc L (Uprod A 𝓤) :=
-  ⟨UprodStruc A (fun _ => strucVal _ _) 𝓤⟩
-
-variable [(ι : I) → CStruc L (A ι)]
-
 lemma realize_Uprod {σ : Sentence L} :
-    Semantics.realize (self := semantics) (UprodStruc A s 𝓤) σ ↔ {ι | Semantics.realize (self := semantics) (s ι) σ} ∈ 𝓤 :=
+    (Uprod A 𝓤) ⊧₁ σ ↔ {ι | Semantics.realize (self := semantics) (s ι) σ} ∈ 𝓤 :=
   by simp[realize_def, SubFormula.val_Uprod, Empty.eq_elim]
 
 variable (A)
 
-def SubFormula.domain (σ : Sentence L) := {ι | (A ι) ⊧ σ}
+def SubFormula.domain (σ : Sentence L) := {ι | (A ι) ⊧₁ σ}
 
 end FirstOrder
 
@@ -118,12 +114,12 @@ variable {L : Language.{u}} {T : CTheory L}
 
 abbrev FinSubTheory (T : CTheory L) := {t : Finset (Sentence L) // ↑t ⊆ T}
 
-variable (A : FinSubTheory T → Type u) (s : (ι : FinSubTheory T) → Structure₁ L (A ι))
+variable (A : FinSubTheory T → Type u) [s : (ι : FinSubTheory T) → Structure₁ L (A ι)]
 
 instance : Inhabited (FinSubTheory T) := ⟨∅, by simp⟩
 
 attribute [instance] Classical.propDecidable in
-lemma ultrafilter_exists (H : ∀ (ι : FinSubTheory T), (A ι) ⊧* (ι.val : CTheory L)) :
+lemma ultrafilter_exists (H : ∀ (ι : FinSubTheory T), (A ι) ⊧₁* (ι.val : CTheory L)) :
     ∃ 𝓤 : Ultrafilter (FinSubTheory T), Set.image (SubFormula.domain A) T ⊆ 𝓤.sets :=
   Ultrafilter.exists_ultrafilter_of_finite_inter_nonempty _ (by
     simp[Finset.subset_image_iff, SubFormula.domain]
@@ -133,16 +129,17 @@ lemma ultrafilter_exists (H : ∀ (ι : FinSubTheory T), (A ι) ⊧* (ι.val : C
     exact H ⟨t, ht⟩ hσ)
 
 theorem compactness :
-  Semantics.Satisfiableₛ T ↔ ∀ ι : FinSubTheory T, Semantics.Satisfiableₛ (ι.val : CTheory L) :=
-  ⟨by rintro h ⟨t, ht⟩; exact Semantics.satisfiableₛ_of_subset h ht,
-   by intro h
-      have : ∀ ι : FinSubTheory T, ∃ (M : Type u) (_ : Inhabited M) (_ : Structure₁ L M), M ⊧* (ι.val : CTheory L) := 
-        by intro ι; exact satisfiableₛ_iff.mp (h ι)
-      choose A si s hA using this
-      have : ∃ 𝓤 : Ultrafilter (FinSubTheory T), Set.image (SubFormula.domain A) T ⊆ 𝓤.sets := ultrafilter_exists A hA
-      rcases this with ⟨𝓤, h𝓤⟩
-      have : Structure₁.Uprod A 𝓤 ⊧* T := by intro σ hσ; exact model_Uprod.mpr (h𝓤 $ Set.mem_image_of_mem (SubFormula.domain A) hσ)
-      exact Semantics.satisfiableₛ_intro (Structure₁.Uprod A 𝓤) this⟩
+    Semantics.Satisfiableₛ T ↔ ∀ ι : FinSubTheory T, Semantics.Satisfiableₛ (ι.val : CTheory L) := by
+  constructor
+  · rintro h ⟨t, ht⟩; exact Semantics.satisfiableₛ_of_subset h ht
+  · intro h
+    have : ∀ ι : FinSubTheory T, ∃ (M : Type u) (_ : Inhabited M) (_ : Structure₁ L M), M ⊧₁* (ι.val : CTheory L) := 
+      by intro ι; exact satisfiableₛ_iff.mp (h ι)
+    choose A si s hA using this
+    have : ∃ 𝓤 : Ultrafilter (FinSubTheory T), Set.image (SubFormula.domain A) T ⊆ 𝓤.sets := ultrafilter_exists A hA
+    rcases this with ⟨𝓤, h𝓤⟩
+    have : Structure₁.Uprod A 𝓤 ⊧₁* T := by intro σ hσ; exact realize_Uprod.mpr (h𝓤 $ Set.mem_image_of_mem (SubFormula.domain A) hσ)
+    exact satisfiableₛ_intro (Structure₁.Uprod A 𝓤) this
 
 end FirstOrder
 
