Logic/Vorspiel/Logic.lean
@@ -3,7 +3,7 @@ import Logic.Vorspiel.Vorspiel
 @[reducible]
 class Semantics (F : Type u) [HasLogicSymbols F] where
   struc : Type w → Type v
-  realize : {M : Type w} → outParam (struc M) → F →L Prop
+  realize : {M : Type w} → struc M → F →L Prop
 
 namespace Semantics
 variable {F : Type u} [HasLogicSymbols F] [s : Semantics.{u, v, w} F]
@@ -11,63 +11,28 @@ variable {F : Type u} [HasLogicSymbols F] [s : Semantics.{u, v, w} F]
 def realizeTheory {M : Type w} (s : struc F M) (T : Set F) : Prop :=
     ∀ ⦃f⦄, f ∈ T → realize s f
 
-@[reducible] class CStruc (F : Type u) [HasLogicSymbols F] [s : Semantics.{u, v, w} F] (M : Type w) where
-  out : s.struc M
+postfix:max " ⊧ₛ " => realize
 
-lemma CStruc.out_mk (x : s.struc M) : CStruc.out (self := CStruc.mk x) = x := rfl
-
-lemma CStruc.mk_out (x : CStruc F M) : CStruc.mk (CStruc.out (self :=  x)) = x := rfl
-
-instance : Coe (struc F M) (CStruc F M) := ⟨CStruc.mk⟩
-
-def models (M : Type w) [c : CStruc F M] : F →L Prop := realize (CStruc.out : s.struc M)
-
-postfix:max " ⊧ " => models
-
-def modelsTheory (M : Type w) [CStruc F M] (T : Set F) : Prop :=
-    ∀ ⦃f⦄, f ∈ T → M ⊧ f
-
-infix:55 " ⊧* " => modelsTheory
+infix:55 " ⊧ₛ* " => realizeTheory
 
 def consequence (T : Set F) (f : F) : Prop :=
-    ∀ (M : Type w) [Inhabited M] [CStruc F M], M ⊧* T → M ⊧ f
+    ∀ (M : Type w) [Inhabited M] (s : struc F M), s ⊧ₛ* T → s ⊧ₛ f
 
 -- note that ⊨ (\vDash) is *NOT* ⊧ (\models)
 infix:55 " ⊨ " => consequence
 
-def Valid (f : F) : Prop := ∀ (M : Type w) [Inhabited M] (_ : CStruc F M), M ⊧ f
+def Valid (f : F) : Prop := ∀ ⦃M : Type w⦄ [Inhabited M] (s : struc F M), s ⊧ₛ f
 
-def Validₛ (T : Set F) : Prop := ∀ (M : Type w) (_ : Inhabited M) (_ : CStruc F M), M ⊧* T
+def Validₛ (T : Set F) : Prop := ∀ ⦃M : Type w⦄ [Inhabited M] (s : struc F M), s ⊧ₛ* T
 
-def Satisfiable (f : F) : Prop := ∃ (M : Type w) (_ : Inhabited M) (_ : CStruc F M), M ⊧ f
+def Satisfiable (f : F) : Prop := ∃ (M : Type w) (_ : Inhabited M) (s : struc F M), s ⊧ₛ f
 
-def Satisfiableₛ (T : Set F) : Prop := ∃ (M : Type w) (_ : Inhabited M) (_ : CStruc F M), M ⊧* T
+def Satisfiableₛ (T : Set F) : Prop := ∃ (M : Type w) (_ : Inhabited M) (s : struc F M), s ⊧ₛ* T
 
-lemma models_iff_models {M : Type w} [CStruc F M] (f : F) :
-    M ⊧ f ↔ realize (CStruc.out : s.struc M) f := of_eq rfl
+lemma valid_neg_iff (f : F) : Valid (~f) ↔ ¬Satisfiable f := by simp[Valid, Satisfiable]
 
-lemma modelsTheory_def {M : Type w} [CStruc F M] (T : Set F) :
-    M ⊧* T ↔ ∀ ⦃f⦄, f ∈ T → realize (CStruc.out : s.struc M) f := of_eq rfl
-
-lemma consequence_iff {T : Set F} {f : F} :
-    T ⊨ f ↔ ∀ (M : Type w) [Inhabited M] (s : struc F M), realizeTheory s T → realize s f := by
-  simp[consequence, models, modelsTheory]; constructor
-  · intro H M i s h; exact @H M i ⟨s⟩ h
-  · intro H M i ⟨s⟩ h; exact @H M i s h 
-
-lemma satisfiableₛ_iff {T : Set F} :
-    Satisfiableₛ T ↔ ∃ (M : Type w) (_ : Inhabited M) (s : struc F M), realizeTheory s T := by
-  simp[Satisfiableₛ, models, modelsTheory]; constructor
-  · intro ⟨M, i, ⟨s⟩, h⟩; exact ⟨M, i, s, h⟩
-  · intro ⟨M, i, s, h⟩; exact ⟨M, i, ⟨s⟩, h⟩
-
-lemma outid_neg (f : F) : Valid (~f) ↔ ¬Satisfiable f := by simp[Valid, Satisfiable]
-
-lemma modelsTheoryₛ_of_subset {T U : Set F} [CStruc F M] (h : M ⊧* U) (ss : T ⊆ U) : M ⊧* T :=
+lemma modelsTheoryₛ_of_subset {T U : Set F} {s : struc F M} (h : s ⊧ₛ* U) (ss : T ⊆ U) : s ⊧ₛ* T :=
   fun _ hf => h (ss hf)
-
-lemma satisfiableₛ_intro {T : Set F} (M : Type w) [i : Inhabited M] [s : CStruc F M] (h : M ⊧* T) : Satisfiableₛ T :=
-  ⟨M, i, s, h⟩
 
 lemma satisfiableₛ_of_subset {T U : Set F} (h : Satisfiableₛ U) (ss : T ⊆ U) : Satisfiableₛ T :=
   by rcases h with ⟨M, i, s, h⟩; exact ⟨M, i, s, modelsTheoryₛ_of_subset h ss⟩
